proof/invariant-abstract/ARM/ArchVSpaceEntries_AI.thy
@@ -1541,7 +1541,7 @@ lemma arch_decode_invocation_valid_pdpt[wp]:
 qed
 
 lemma decode_invocation_valid_pdpt[wp]:
-  "\<lbrace>invs and valid_cap cap and valid_pdpt_objs\<rbrace> 
+  "\<lbrace>invs and valid_cap cap and valid_pdpt_objs\<rbrace>
      decode_invocation label args cap_index slot cap excaps
    \<lbrace>invocation_duplicates_valid\<rbrace>,-"
   apply (simp add: decode_invocation_def split del: if_split)
